# Part 1
### Failure Inducing Input JUnit Test
```
public void testReversed2() {
    int[] input1 = {1, 2, 3};
    assertArrayEquals(new int[]{3, 2, 1}, ArrayExamples.reversed(input1));
  }
```
### Associated Code (from ArrayExamples)
```
static int[] reversed(int[] arr) {
    int[] newArray = new int[arr.length];
    for(int i = 0; i < arr.length; i += 1) {
      arr[i] = newArray[arr.length - i - 1];
    }
    return arr;
  }
```

### Non-failure inducing Input JUnit Test
```
@Test
  public void testReversed() {
    int[] input1 = { };
    assertArrayEquals(new int[]{ }, ArrayExamples.reversed(input1));
  }
```
### Output
![image](lab3part1output)

### Bug Before Code
```
static int[] reversed(int[] arr) {
    int[] newArray = new int[arr.length];
    for(int i = 0; i < arr.length; i += 1) {
      arr[i] = newArray[arr.length - i - 1];
    }
    return arr;
  }
```
### Bug After Code-Fix
```
static int[] reversed(int[] arr) {
    int[] newArray = new int[arr.length];
    for(int i = 0; i < arr.length; i += 1) {
      newArray[i] = arr[arr.length - i - 1];
    }
    return newArray;
  }
```
* This fix addresses the bug in the `reversed()` method because the previous method put the zero elements from the new array to the old array, which should be the opposite where we put the elements from the back of the original list into the beginning of the new array, returning this new array instead of the old one
